finish copy array

scratch/Scratch_CopyArray.thy
@@ -2,48 +2,56 @@ theory Scratch_CopyArray
   imports Refine_Imperative_HOL.IICF
 begin
 
-definition fill_one :: "int list \<Rightarrow> int list nres" where
-  "fill_one l \<equiv> RETURN (map (\<lambda>_. 1) l)"
+definition fill_one_spec :: "int list \<Rightarrow> int list nres" where
+  "fill_one_spec l \<equiv> RETURN (map (\<lambda>_. 1) l)"
 
 definition fill_one1 :: "int list \<Rightarrow> int list nres" where
   "fill_one1 l \<equiv> RETURN (fold (\<lambda>i l. (list_update l i 1)) [0..<length l] l)"
 
-lemma "(fill_one1, fill_one) \<in> Id \<rightarrow> \<langle>Id\<rangle>nres_rel"
-proof -
-  { fix l :: "int list"
-    have fix_len[simp]: "x \<le> length l \<Longrightarrow> length (fold (\<lambda>i l. (list_update l i 1)) [0..<x] l) = length l" for x
-      by (induction x) auto
-    have "x \<le> length l \<Longrightarrow> take x (fold (\<lambda>i l. (list_update l i 1)) [0..<x] l) = replicate x 1" for x
-      by (induction x) (auto simp: take_update_last replicate_append_same)
-    note this[of "length l", simplified, folded map_replicate_const]
-  }
-  thus ?thesis
-    unfolding fill_one_def fill_one1_def
-    by refine_vcg auto
-qed
+lemma fold_fix_length: "x \<le> length l \<Longrightarrow> length (fold (\<lambda>i l. (list_update l i 1)) [0..<x] l) = length l"
+  by (induction x) auto
 
-sepref_definition fill_one2 is fill_one1 :: "(array_assn int_assn)\<^sup>d \<rightarrow>\<^sub>a (array_assn int_assn)"
-  unfolding fill_one1_def
-  apply sepref_dbg_keep
-      apply sepref_dbg_trans_keep
-          apply sepref_dbg_trans_step_keep
-  apply (sepref_dbg_side_keep)
-  term 0(*          apply sepref_dbg_trans_step_keep
-         apply sepref_dbg_trans_step_keep
-           apply sepref_dbg_trans_step_keep
-          apply sepref_dbg_trans_step_keep
-         apply sepref_dbg_trans_step_keep
-        apply sepref_dbg_trans_step_keep
-       apply sepref_dbg_trans_step_keep
-              apply sepref_dbg_trans_step_keep
-             apply sepref_dbg_trans_step_keep
-            apply sepref_dbg_trans_step_keep
-           apply sepref_dbg_trans_step_keep
-          apply sepref_dbg_trans_step_keep
-         apply sepref_dbg_trans_step_keep
-           apply sepref_dbg_trans_step_keep
-          apply sepref_dbg_trans_step_keep
-          apply sepref_dbg_trans_step_keep
-          apply sepref_dbg_trans_step_keep
-  
+lemma fill_replicate_partial: "x \<le> length l \<Longrightarrow> take x (fold (\<lambda>i l. (list_update l i 1)) [0..<x] l) = replicate x 1" for x
+  by (induction x) (auto simp: take_update_last replicate_append_same fold_fix_length)
+
+corollary fill_replicate: "fold (\<lambda>i l. (list_update l i 1)) [0..<length l] l = replicate (length l) 1"
+  using fill_replicate_partial by (fastforce simp: fold_fix_length)
+
+corollary fill_length_cong:
+  assumes "length l0 = length l1"
+  shows "fold (\<lambda>i l. (list_update l i 1)) [0..<length l0] l1 = replicate (length l1) 1"
+  unfolding assms fill_replicate ..
+
+lemma fill_one1_refine: "(fill_one1, fill_one_spec) \<in> Id \<rightarrow> \<langle>Id\<rangle>nres_rel"
+  unfolding fill_one_spec_def fill_one1_def
+  apply (refine_vcg)
+  apply (vc_solve simp: fill_replicate map_replicate_const)
+  done
+
+definition fill_one2 :: "int list \<Rightarrow> int list nres" where
+  "fill_one2 l \<equiv> nfoldli [0..<length l] (\<lambda>_. True) (\<lambda>i l'. ASSERT (i < length l') \<then> RETURN (list_update l' i 1)) l"
+
+lemma fill_one2_refine: "(fill_one2, fill_one1) \<in> Id \<rightarrow> \<langle>Id\<rangle>nres_rel"
+  unfolding fill_one2_def fill_one1_def
+  apply (refine_vcg nfoldli_rule[where I="\<lambda>l1 l2 l. take (length l1) l = replicate (length l1) 1 \<and> length l1 + length l2 = length l"])
+        apply (vc_solve simp: upt_eq_lel_conv take_update_last replicate_append_same fill_length_cong)
+  done
+
+sepref_definition fill_one3 is fill_one2 :: "(array_assn int_assn)\<^sup>d \<rightarrow>\<^sub>a (array_assn int_assn)"
+  unfolding fill_one2_def
+  by sepref
+
+
+lemmas fill_one3_correct = fill_one3.refine[FCOMP fill_one2_refine, FCOMP fill_one1_refine]
+
+lemma fill_one2_refine': "(fill_one2, fill_one_spec) \<in> Id \<rightarrow> \<langle>Id\<rangle>nres_rel"
+  unfolding fill_one2_def fill_one_spec_def
+  apply (refine_vcg nfoldli_rule[where I="\<lambda>l1 l2 l. l = map (\<lambda>_. 1) (take (length l1) l) @ drop (length l1) l \<and> length l = length l1 + length l2"])
+        apply (vc_solve simp: upt_eq_lel_conv replicate_append_same[symmetric] map_replicate_const upd_conv_take_nth_drop)
+  subgoal premises prems
+    apply (rewrite prems(1))
+    apply simp
+    done
+  done
+
 end
